WIP

MPL/ProofMode/Tactics/VCGen.lean
@@ -23,11 +23,103 @@ import MPL.Triple
 namespace MPL.ProofMode.Tactics
 open Lean Elab Tactic Meta
 
+initialize registerTraceClass `mpl.tactics.vcgen
 
+namespace VC
 
-elab "mvcgen" : tactic => do
+def step (goal : MGoal) (subst : Array Expr) (discharge : MGoal → Array Expr → MetaM Expr) : MetaM Expr := do
+  let T := goal.target.consumeMData
+  trace[mpl.tactics.vcgen] "target: {T}"
+  logInfo m!"target: {T}"
+  if let some _ := T.app3? ``SPred.imp then
+    return ← mIntro goal (← `(binderIdent| _)) (fun g => discharge g subst)
+  if T.isAppOf ``PredTrans.apply then
+    let args := T.getAppArgs
+    let wp := args[2]!
+    let Q := args[3]!
+    match_expr wp with
+    | WP.wp m ps instWP α e =>
+      let us := wp.getAppFn.constLevels!
+      if let .letE x ty val body _nonDep := e then
+        return ← withLetDecl x ty val fun fv => do
+        let subst := subst.push fv
+        let wp' := mkApp5 (mkConst ``WP.wp us) m ps instWP α body
+        let args' := args.set! 2 wp'
+        let goal := { goal with target := mkAppN (mkConst ``PredTrans.apply) args' }
+        mkLetFVars #[fv] (← discharge goal subst)
+      logInfo m!"hyps: {(← getLocalHyps)}"
+      logInfo m!"e: {e}"
+      if e.isIte then
+        let ite_args := e.getAppArgs
+        -- TODO: Only do this if Q is not already a var
+        let Qty := mkApp2 (mkConst ``PostCond) α ps
+        return ← withLetDecl `Q Qty Q fun Q => do
+        let t := mkApp5 (mkConst ``WP.wp us) m ps instWP α (e.getArg! 3)
+        let e := mkApp5 (mkConst ``WP.wp us) m ps instWP α (e.getArg! 4)
+        let tapplyQ := mkAppN (mkConst ``PredTrans.apply) (args.set! 2 t |>.set! 3 Q)
+        let eapplyQ := mkAppN (mkConst ``PredTrans.apply) (args.set! 2 e |>.set! 3 Q)
+        let ret_ty := (← inferType tapplyQ)
+        let u ← getLevel ret_ty
+        let ite_args' := ite_args.set! 0 (← inferType tapplyQ) |>.set! 3 tapplyQ |>.set! 4 eapplyQ
+        let ite := mkAppN (mkConst ``ite [u]) ite_args'
+        let goal := { goal with target := ite }
+        mkLetFVars #[Q] (← discharge goal subst)
+      if e.isAppOf ``Pure.pure then
+        return ← withLetDecl `a α (e.getArg! 3) fun a => do
+        let goal := { goal with target := mkAppN (mkApp (mkProj ``Prod 0 Q) a) args }
+        mkLetFVars #[a] (← discharge goal subst)
+      -- Split match-expressions
+      if let some info := isMatcherAppCore? (← getEnv) e then
+        let candidate ← id do
+          let args := e.getAppArgs
+          logInfo "e: {e}, args: {args}"
+          for i in [info.getFirstDiscrPos : info.getFirstDiscrPos + info.numDiscrs] do
+            if args[i]!.hasLooseBVars then
+              return false
+          return true
+        if candidate then
+          -- We could be even more deliberate here and use the `lifter` lemmas
+          -- for the match statements instead of the `split` tactic.
+          -- For now using `splitMatch` works fine.
+          -- return ← Split.splitMatch goal e
+          return ← discharge goal subst
+    | _ => return ← discharge goal subst
+--    if wp.isAppOf ``WP.wp then
+--      let_expr WP.wp m ps instWP α x := wp | throwError "target not a wp application {wp}"
+--    match
+  return ← discharge goal subst
+
+partial def loop (goal : MGoal) (subst : Array Expr) (discharge : MGoal → Array Expr → MetaM Expr) : MetaM Expr := do
+  VC.step goal subst fun hyp subst' => do
+    logInfo m!"goal: {goal.toExpr}, hyp: {hyp.toExpr}"
+    if subst.size = subst'.size && (← isDefEq goal.toExpr hyp.toExpr) then
+      return ← discharge hyp subst'
+    return ← discharge hyp subst'
+    --loop goal subst' discharge
+
+end VC
+
+elab "mvcgen_step" : tactic => do
   let (mvar, goal) ← mStart (← getMainGoal)
-  replaceMainGoal mvars
+  mvar.withContext do
+  let goals ← IO.mkRef []
+  mvar.assign (← VC.step goal #[] fun hyp subst => do
+    let m ← mkFreshExprSyntheticOpaqueMVar (hyp.toExpr.instantiateRev subst)
+    goals.modify (m.mvarId! :: ·)
+    return m)
+  replaceMainGoal (← goals.get)
+
+elab "mvcgen'" : tactic => do
+  let (mvar, goal) ← mStart (← getMainGoal)
+  mvar.withContext do
+  let goals ← IO.mkRef []
+  mvar.assign (← VC.loop goal #[] fun hyp subst => do
+    let m ← mkFreshExprSyntheticOpaqueMVar (hyp.toExpr.instantiateRev subst)
+    goals.modify (m.mvarId! :: ·)
+    return m)
+  replaceMainGoal (← goals.get)
+
+macro "mvcgen" : tactic => `(tactic| repeat mvcgen_step)
 
 def fib_impl (n : Nat) : Idd Nat := do
   if n = 0 then return 0
@@ -57,8 +149,12 @@ theorem fib_triple : ⦃⌜True⌝⦄ fib_impl n ⦃⇓ r => r = fib_spec n⦄ :
 
 theorem fib_triple_vc : ⦃⌜True⌝⦄ fib_impl n ⦃⇓ r => r = fib_spec n⦄ := by
   unfold fib_impl
-  mstart
-  mvcgen
+  mvcgen'
+  mvcgen_step
+  intro h
+  mvcgen_step
+  mvcgen_step
+  mvcgen_step
 --  dsimp
 --  mintro _
 --  if h : n = 0 then simp [h] else
